moved commands to stack frame

src/return.c
@@ -1,0 +1,16 @@
+void f() {
+  
+}
+
+int g(int x) {
+  if (x<0) return 1;
+  while (1+x) {
+    
+    
+  }
+}
+
+int main() {
+  f();
+  return 0;
+}
