src/Com.thy
@@ -4,7 +4,7 @@ begin
 
 type_synonym fname = string
 
-datatype
+datatype_new
   com = SKIP
       | Assignl lexp exp       ("_ ::== _" [1000, 61] 61)
       | Assign  vname exp      ("_ ::= _" [1000, 61] 61)
@@ -12,18 +12,26 @@ datatype
       | If      exp com com    ("(IF _/ THEN _/ ELSE _)"  [0, 0, 61] 61)
       | While   exp com        ("(WHILE _/ DO _)"  [0, 61] 61)
       | Free    lexp           ("FREE _" [0])
-      | Return exp
+      | is_Return: Return exp
       | Callfunl lexp fname "exp list" ("_ ::== _ '(_')" [1000, 61] 61)
       | Callfun vname fname "exp list" ("_ ::= _ '(_')" [1000, 61] 61)
-      | Block com
+      (*| Block com*)
 
 term "''x'' ::= ''fun'' ([])"
 term "(Derefl (V ''x'')) ::== ''fun'' ([])"
 
 type_synonym fun_decl = "vname list \<times> vname list \<times> com"
 
+fun def_returns :: "com \<Rightarrow> bool" where
+  "def_returns (Return _) \<longleftrightarrow> True"
+| "def_returns (c1 ;; c2) \<longleftrightarrow> def_returns c1 \<or> def_returns c2"
+| "def_returns (IF _ THEN c1 ELSE c2) \<longleftrightarrow> def_returns c1 \<and> def_returns c2"
+| "def_returns _ \<longleftrightarrow> False"
+
 fun valid_fun_decl :: "fun_decl \<Rightarrow> bool" 
-  where "valid_fun_decl (params,locals,com) \<longleftrightarrow> distinct (params @ locals)"
+  where "valid_fun_decl (params,locals,com) \<longleftrightarrow> 
+    distinct (params @ locals)
+  \<and> def_returns com"
 
 type_synonym program = "fname \<Rightarrow> fun_decl option"
 
